src/Narcissus/Automation/AlignedAutomation.v
@@ -1,4 +1,6 @@
-
+Require Import Fiat.Narcissus.BinLib
+        Fiat.Narcissus.Common.Specs
+        Fiat.Narcissus.Automation.Solver.
 
 Ltac start_synthesizing_encoder :=
   lazymatch goal with
@@ -9,11 +11,49 @@ Ltac start_synthesizing_encoder :=
   (*pose_string_hyps; *)
   eexists; simpl; intros.
 
+Ltac align_encoder_step :=
+  first [
+      apply @CorrectAlignedEncoderForThenC
+    | apply @CorrectAlignedEncoderForDoneC
+    | apply CorrectAlignedEncoderForFormatList
+    | apply CorrectAlignedEncoderForFormatChar; eauto
+    | apply CorrectAlignedEncoderForFormat2Char; eauto
+    | apply CorrectAlignedEncoderForFormatNat].
+
 Ltac align_encoder :=
-    repeat first [
-           apply @CorrectAlignedEncoderForThenC
-         | apply @CorrectAlignedEncoderForDoneC
-         | apply CorrectAlignedEncoderForFormatList
-         | apply CorrectAlignedEncoderForFormatChar; eauto
-         | apply CorrectAlignedEncoderForFormat2Char; eauto
-         | apply CorrectAlignedEncoderForFormatNat].
+  repeat align_encoder_step.
+
+Ltac start_synthesizing_decoder :=
+  match goal with
+  | |- CorrectAlignedDecoderFor ?Invariant ?Spec =>
+    try unfold Spec; try unfold Invariant
+  end;
+
+  (* Memoize any string constants *)
+  (* pose_string_hyps; *)
+  eapply Start_CorrectAlignedDecoderFor; simpl; intros.
+
+Ltac align_decoders_step :=
+  first [
+      eapply @AlignedDecodeNatM; intros
+    | eapply @AlignedDecodeBind2CharM; intros; eauto
+    | eapply @AlignedDecodeListM; intros; eauto
+    | eapply @AlignedDecodeCharM; intros; eauto
+    | eapply @Return_DecodeMEquivAlignedDecodeM].
+
+Ltac align_decoders := repeat align_decoders_step.
+Locate Ltac normalize_compose .
+Ltac synthesize_aligned_decoder :=
+  start_synthesizing_decoder;
+  [ match goal with
+      |- CorrectDecoder ?monoid _ _ _ _ _ => normalize_compose monoid
+    end;
+    repeat decode_step idtac
+  | cbv beta; synthesize_cache_invariant
+  | cbv beta; optimize_decoder_impl
+  | ];
+  cbv beta; align_decoders.
+
+Ltac synthesize_aligned_encoder :=
+  start_synthesizing_encoder;
+  align_encoder.
