src/Narcissus/BinLib.v
@@ -1,3 +1,7 @@
+Require Import Fiat.Narcissus.Common.Monoid.
+
+Require Import Bedrock.Word.
+
 Require Export
         Fiat.Narcissus.BinLib.AlignedByteString
         Fiat.Narcissus.BinLib.AlignWord
@@ -7,3 +11,11 @@ Require Export
         Fiat.Narcissus.BinLib.AlignedEncodeMonad.
 
 Global Instance ByteStringQueueMonoid : Monoid ByteString := ByteStringQueueMonoid.
+
+(* Various Constants that clients should never simplify. *)
+Global Arguments split1 : simpl never.
+Global Arguments split2 : simpl never.
+Global Arguments weq : simpl never.
+Global Arguments natToWord : simpl never.
+Global Arguments Guarded_Vector_split : simpl never.
+Global Arguments Core.append_word : simpl never.
